Proving the expected basic equations for the para combinator

examples/CCS/Denotation.v
@@ -63,8 +63,8 @@ Definition ccsE : Type -> Type := ActionE.
 Definition ccsT' T := ctree' ccsE T.
 Definition ccsT := ctree ccsE.
 
-Definition ccs' := ccsT' unit.
-Definition ccs  := ccsT unit.
+Definition ccs' := ccsT' void.
+Definition ccs  := ccsT void.
 
 (*| Process algebra |*)
 Section Combinators.
@@ -148,8 +148,8 @@ Unless one is silent stuck, the other visible stuck...
         (rQ <- get_head Q;;
          match rQ with
          | HRet rQ => stuckI
-         | HChoice kQ => ChoiceV _ (fun i => F (kQ i) Q)
-         | HVis e kQ => Vis e (fun i => F (kQ i) Q)
+         | HChoice kQ => ChoiceV _ (fun i => F P (kQ i))
+         | HVis e kQ => Vis e (fun i => F P (kQ i))
          end)
 
         (rP <- get_head P;;
@@ -303,6 +303,416 @@ bang p = get_head P ;;
 
 End Combinators.
 
+Definition comm a : label := obs (Act a) tt.
+Notation "0" := nil: ccs_scope.
+Infix "+" := plus (at level 50, left associativity).
+(* Infix "∥" := communicating (at level 29, left associativity). *)
+Infix "∥" := para (at level 29, left associativity).
+
+Notation para_ p q :=
+  (choiceI3
+    (rp <- get_head p;;
+     match rp with
+     | HRet rp => stuckI
+     | HChoice kp => ChoiceV _ (fun i => para (kp i) q)
+     | HVis e kp => Vis e (fun i => para (kp i) q)
+     end)
+
+    (rq <- get_head q;;
+     match rq with
+     | HRet rq => stuckI
+     | HChoice kq => ChoiceV _ (fun i => para p (kq i))
+     | HVis e kq => Vis e (fun i => para p (kq i))
+     end)
+
+    (rp <- get_head p;;
+     rq <- get_head q;;
+     match rp, rq with
+     | HVis ep kp, HVis eq kq =>
+         match ep, kp, eq, kq with
+         | Act a, kp, Act b, kq =>
+             if are_opposite a b
+             then
+               TauV (para (kp tt) (kq tt))
+             else
+               stuckI
+         end
+     | _, _ => stuckI
+     end))%ctree.
+
+Lemma unfold_para : forall p q, para p q ≅ para_ p q.
+Proof.
+  intros.
+	now step.
+Qed.
+
+#[global] Instance para_equ :
+  Proper (equ eq ==> equ eq ==> equ eq) para.
+Proof.
+  unfold Proper, respectful.
+  coinduction R CIH.
+  intros p1 p2 EQp q1 q2 EQq.
+  rewrite 2 unfold_para.
+  constructor.
+  intros i.
+  destruct i; [| destruct i].
+  - eapply (ft_t (bind_ctx_equ_t _ _)).
+    apply in_bind_ctx; [apply get_head_equ; auto | intros hdp1 hdp2 eqp].
+    inv eqp; auto.
+    step; constructor; auto.
+    step; constructor; auto.
+  - eapply (ft_t (bind_ctx_equ_t _ _)).
+    apply in_bind_ctx; [apply get_head_equ; auto | intros hdp1 hdp2 eqp].
+    inv eqp; auto.
+    step; constructor; auto.
+    step; constructor; auto.
+  - eapply (ft_t (bind_ctx_equ_t _ _)).
+    apply in_bind_ctx; [apply get_head_equ; auto | intros hdp1 hdp2 eqp].
+    eapply (ft_t (bind_ctx_equ_t _ _)).
+    apply in_bind_ctx; [apply get_head_equ; auto | intros hdq1 hdq2 eqq].
+    inv eqp; auto.
+    inv eqq; auto.
+    destruct e, e0, (are_opposite a a0); auto.
+    step; constructor; auto.
+Qed.
+
+Lemma trans_choiceI31 :
+  forall {E X} (t t' u v : ctree E X) l,
+    trans l t t' ->
+    trans l (choiceI3 t u v) t'.
+Proof.
+  intros * TR.
+  eapply trans_ChoiceI with (x := Fin.F1); eauto.
+Qed.
+
+Lemma trans_choiceI32 :
+  forall {E X} (t u u' v : ctree E X) l,
+    trans l u u' ->
+    trans l (choiceI3 t u v) u'.
+Proof.
+  intros * TR.
+  eapply trans_ChoiceI with (x := Fin.FS Fin.F1); eauto.
+Qed.
+
+Lemma trans_choiceI33 :
+  forall {E X} (t u v v' : ctree E X) l,
+    trans l v v' ->
+    trans l (choiceI3 t u v) v'.
+Proof.
+  intros * TR.
+  eapply trans_ChoiceI with (x := Fin.FS (Fin.FS Fin.F1)); eauto.
+Qed.
+
+Lemma trans_ChoiceV' {E X} : forall n (k : fin n -> ctree E X) x u,
+    u ≅ k x ->
+		trans tau (ChoiceV n k) u.
+Proof.
+	intros * eq; rewrite eq; apply trans_ChoiceV.
+Qed.
+
+Lemma trans_paraSynch : forall a b (p p' q q' : ccs),
+    trans (comm a) p p' ->
+    trans (comm b) q q' ->
+    are_opposite a b ->
+    trans tau (p ∥ q) (p' ∥ q').
+Proof.
+  intros * TRp TRq Op.
+  apply trans_get_head in TRp as (kp & TRp & Eqp).
+  apply trans_get_head in TRq as (kq & TRq & Eqq).
+  rewrite unfold_para.
+  apply trans_choiceI33.
+  eapply trans_bind_r; [apply TRp |].
+  eapply trans_bind_r; [apply TRq |].
+  cbn; rewrite Op.
+  rewrite Eqp, Eqq.
+  apply trans_TauV.
+Qed.
+
+Lemma trans_paraL :
+  forall l (p p' q : ccs),
+    trans l p p' ->
+    trans l (p ∥ q) (p' ∥ q).
+Proof.
+  intros * TRp.
+  rewrite unfold_para.
+  apply trans_choiceI31.
+  destruct l.
+  - apply trans_get_head in TRp.
+    destruct TRp as (? & ? & ? & TRp & Eqp).
+    eapply trans_bind_r; eauto; cbn.
+    econstructor.
+    rewrite Eqp; reflexivity.
+  - apply trans_get_head in TRp.
+    destruct TRp as (? & TRp & Eqp).
+    eapply trans_bind_r; eauto; cbn.
+    constructor.
+    rewrite Eqp; reflexivity.
+  - pose proof (trans_val_invT TRp); subst; easy.
+Qed.
+
+Lemma trans_paraR :
+  forall l (p q q' : ccs),
+    trans l q q' ->
+    trans l (p ∥ q) (p ∥ q').
+Proof.
+  intros * TRq.
+  rewrite unfold_para.
+  apply trans_choiceI32.
+  destruct l.
+  - apply trans_get_head in TRq.
+    destruct TRq as (? & ? & ? & TRq & Eqq).
+    eapply trans_bind_r; eauto; cbn.
+    econstructor.
+    rewrite Eqq; reflexivity.
+  - apply trans_get_head in TRq.
+    destruct TRq as (? & TRq & Eqq).
+    eapply trans_bind_r; eauto; cbn.
+    constructor.
+    rewrite Eqq; reflexivity.
+  - pose proof (trans_val_invT TRq); subst; easy.
+Qed.
+
+Lemma trans_para_inv :
+  forall l p q r,
+    trans l (p ∥ q) r ->
+    (exists p', trans l p p' /\ r ≅ (p' ∥ q)) \/
+    (exists q', trans l q q' /\ r ≅ (p ∥ q')) \/
+    (exists p' q' a b,
+          trans (comm a) p p' /\
+            trans (comm b) q q' /\
+            are_opposite a b /\
+            l = tau /\
+            r ≅ (p' ∥ q')).
+Proof.
+  intros * TR.
+  rewrite unfold_para in TR.
+  apply trans_ChoiceI_inv in TR as (x & TR).
+  destruct x; [| destruct x].
+  - left.
+    edestruct @trans_bind_inv; [apply TR | | ]; clear TR.
+    destruct H as (NOTV & ? & TR & EQ); apply trans_get_head_inv in TR; easy.
+    destruct H as (hdp & TRhdp & TR).
+    destruct hdp; try easy.
+    * apply trans_ChoiceV_inv in TR as (x & EQ & ->).
+      eapply trans_HChoice in TRhdp.
+      eexists; split; eauto.
+    * apply trans_vis_inv in TR as (x & EQ & ->).
+      eapply trans_HVis in TRhdp.
+      eexists; split; eauto.
+  - right; left.
+    edestruct @trans_bind_inv; [apply TR | | ]; clear TR.
+    destruct H as (NOTV & ? & TR & EQ); apply trans_get_head_inv in TR; easy.
+    destruct H as (hdq & TRhdq & TR).
+    destruct hdq; try easy.
+    * apply trans_ChoiceV_inv in TR as (x & EQ & ->).
+      eapply trans_HChoice in TRhdq.
+      eexists; split; eauto.
+    * apply trans_vis_inv in TR as (x & EQ & ->).
+      eapply trans_HVis in TRhdq.
+      eexists; split; eauto.
+  - right; right.
+    edestruct @trans_bind_inv; [apply TR | | ]; clear TR.
+    destruct H as (NOTV & ? & TR & EQ); apply trans_get_head_inv in TR; easy.
+    destruct H as (hdp & TRhdp & TR).
+    edestruct @trans_bind_inv; [apply TR | | ]; clear TR.
+    destruct H as (NOTV & ? & TR & EQ); apply trans_get_head_inv in TR; easy.
+    destruct H as (hdq & TRhdq & TR).
+    destruct hdp; try easy.
+    exfalso; eapply stuckI_is_stuck; eassumption.
+    destruct hdq; try easy.
+    exfalso; eapply stuckI_is_stuck; eassumption.
+    destruct e, e0, (are_opposite a a0) eqn:?.
+    2:exfalso; eapply stuckI_is_stuck; eassumption.
+    apply trans_TauV_inv in TR as [? ->].
+    eapply trans_HVis in TRhdp.
+    eapply trans_HVis in TRhdq.
+    do 4 eexists.
+    repeat split; eauto.
+Qed.
+
+Section Theory.
+
+  Lemma plsC: forall (p q : ccs), p+q ~ q+p.
+  Proof.
+    apply choiceI2_commut.
+  Qed.
+
+  Lemma plsA (p q r : ccs): p+(q+r) ~ (p+q)+r.
+  Proof.
+    symmetry; apply choiceI2_assoc.
+  Qed.
+
+  Lemma pls0p (p : ccs) : 0 + p ~ p.
+  Proof.
+    apply choiceI2_stuckV_l.
+  Qed.
+
+  Lemma plsp0 (p : ccs) : p + 0 ~ p.
+  Proof. now rewrite plsC, pls0p. Qed.
+
+  Lemma plsidem (p : ccs) : p + p ~ p.
+  Proof.
+    apply choiceI2_idem.
+  Qed.
+
+  Ltac trans_para_invT H :=
+    apply trans_para_inv in H as
+        [(?p' & ?TRp & ?EQ) |
+          [(?q' & ?TRq & ?EQ) |
+            (?p' & ?q' & ?a & ?b & ?TRp & ?TRq & ?Op & ? & ?EQ) ]]; subst.
+
+  #[global] Instance are_opposite_sym : Symmetric are_opposite.
+  Proof.
+    unfold are_opposite, eqb_action, op; cbn.
+    intros [] [] Op; intuition.
+    all:rewrite eqb_sym; auto.
+  Qed.
+
+  Lemma paraC: forall (p q : ccs), p ∥ q ~ q ∥ p.
+  Proof.
+    coinduction ? CIH; symmetric.
+    intros p q l r tr.
+    trans_para_invT tr.
+    - eexists.
+      eapply trans_paraR; eauto.
+      rewrite EQ; auto.
+    - eexists.
+      eapply trans_paraL; eauto.
+      rewrite EQ; auto.
+    - eexists.
+      eapply trans_paraSynch; eauto.
+      symmetry; auto.
+      rewrite EQ; auto.
+  Qed.
+
+  Lemma para0p : forall (p : ccs), 0 ∥ p ~ p.
+  Proof.
+    coinduction R CIH.
+    intros.
+    split.
+    - intros l q tr.
+      trans_para_invT tr; try now exfalso; eapply stuckV_is_stuck; eauto.
+      eexists; eauto.
+      rewrite EQ; auto.
+    - intros l q tr.
+      eexists.
+      apply trans_paraR; eauto.
+      cbn; auto.
+  Qed.
+
+  Lemma parap0 : forall (p : ccs), p ∥ 0 ~ p.
+  Proof.
+    intros; rewrite paraC; apply para0p.
+  Qed.
+
+  Lemma paraA : forall (p q r : ccs), p ∥ (q ∥ r) ~ (p ∥ q) ∥ r.
+  Proof.
+    coinduction ? CIH; intros.
+    split.
+    - intros l s tr.
+      trans_para_invT tr.
+      + eexists.
+        do 2 apply trans_paraL; eauto.
+        rewrite EQ; auto.
+      + trans_para_invT TRq.
+        * eexists.
+          apply trans_paraL, trans_paraR; eauto.
+          rewrite EQ, EQ0; auto.
+        * eexists.
+          apply trans_paraR; eauto.
+          rewrite EQ, EQ0; auto.
+        * eexists.
+          eapply trans_paraSynch; eauto.
+          eapply trans_paraR; eauto.
+          rewrite EQ, EQ0; auto.
+      + trans_para_invT TRq.
+        * eexists.
+          eapply trans_paraL, trans_paraSynch; eauto.
+          rewrite EQ, EQ0; auto.
+        * eexists.
+          eapply trans_paraSynch; eauto.
+          eapply trans_paraL; eauto.
+          rewrite EQ, EQ0; auto.
+        * inv H.
+    - intros l s tr; cbn.
+      trans_para_invT tr.
+      + trans_para_invT TRp.
+        * eexists.
+          apply trans_paraL; eauto.
+          rewrite EQ, EQ0; auto.
+        * eexists.
+          apply trans_paraR, trans_paraL; eauto.
+          rewrite EQ, EQ0; auto.
+        * eexists.
+          eapply trans_paraSynch; eauto.
+          eapply trans_paraL; eauto.
+          rewrite EQ, EQ0; auto.
+      + eexists.
+        eapply trans_paraR, trans_paraR; eauto.
+        rewrite EQ; auto.
+      + trans_para_invT TRp.
+        * eexists.
+          eapply trans_paraSynch; eauto.
+          eapply trans_paraR; eauto.
+          rewrite EQ, EQ0; auto.
+        * eexists.
+          eapply trans_paraR, trans_paraSynch; eauto.
+          rewrite EQ, EQ0; auto.
+        * inv H.
+  Qed.
+
+End Theory.
+
+Import CCSNotations.
+Open Scope ccs_scope.
+
+(* fun P Q => bisim (model P) (model Q): is this weak bisimulation of CCS?
+
+   -> : term -> term -> Prop
+   -ccs> : ccs -> ccs -> Prop as
+   -sem> : term -> term -> Prop := fun P Q => model P -ccs> model Q
+*)
+
+Fixpoint model (t : term) : ccs :=
+	match t with
+	| 0      => nil
+	| a · P  => prefix a (model P)
+	| TauT P => TauV (model P)
+	| P ∥ Q  => para (model P) (model Q)
+	| P ⊕ Q  => plus (model P) (model Q)
+	| P ∖ c  => restrict c (model P)
+	end.
+
+(*
+Variant step_ccs : ccs -> option action -> ccs -> Prop :=
+| Sted_comm : forall (t : ccs) a u k,
+	schedule t u ->
+  u ≅ trigger (Act a);; k ->
+	step_ccs t (Some a) k
+| Step_tau : forall (t : ccs) u k,
+	schedule t u ->
+  u ≅ trigger Tau;; k ->
+	step_ccs t None k.
+
+Definition step_sem : term -> option action -> term -> Prop :=
+	fun P a Q => step_ccs (model P) a (model Q).
+*)
+
+Module DenNotations.
+
+  (* Notations for patterns *)
+  Notation "'synchP' e" := (inl1 e) (at level 10).
+  Notation "'actP' e" := (inr1 (inl1 e)) (at level 10).
+  Notation "'deadP' e" :=  (inr1 (inr1 e)) (at level 10).
+
+  Notation "⟦ t ⟧" := (model t).
+  (* Notation "P '⊢' a '→ccs' Q" := (step_ccs P a Q) (at level 50). *)
+  (* Notation "P '⊢' a '→sem' Q" := (step_sem P a Q) (at level 50). *)
+
+End DenNotations.
+
+Import DenNotations.
+
 Notation communicating_ P Q :=
 	(rP <- get_head P;;
 	 rQ <- get_head Q;;
@@ -350,9 +760,9 @@ Proof.
   eapply (fbt_bt (bind_ctx_equ_t _ _)).
   apply in_bind_ctx; [apply get_head_equ; auto | intros hdQ1 hdQ2 eqq].
   destruct hdP1, hdP2; try now inv eqp.
-  - rewrite EQQ; reflexivity.
+  (* - rewrite EQQ; reflexivity. *)
   - destruct hdQ1, hdQ2; try now inv eqq.
-    + rewrite EQP; reflexivity.
+    (* + rewrite EQP; reflexivity. *)
     + dependent induction eqp.
       dependent induction eqq.
       constructor.
@@ -366,7 +776,7 @@ Proof.
       step; constructor; auto.
       step; constructor; auto.
   - destruct hdQ1, hdQ2; try now inv eqq.
-    + destruct e,e0; rewrite EQP; reflexivity.
+    (* + destruct e,e0; rewrite EQP; reflexivity. *)
     + dependent induction eqp.
       dependent induction eqq.
       destruct e0.
@@ -405,7 +815,6 @@ Proof.
        preventing any communication from happening *)
 Abort.
 
-Definition comm a : label := obs (Act a) tt.
 Lemma trans_communicatingSynch : forall a b (P P' Q Q' : ccs),
     trans (comm a) P P' ->
     trans (comm b) Q Q' ->
@@ -428,15 +837,13 @@ Lemma trans_communicatingL :
   forall l l' (P P' Q Q' : ccs),
     trans l P P' ->
     trans l' Q Q' ->
-    (trans l (communicating P Q) (communicating P' Q) \/
-       (l' = val tt /\ Q' ≅ stuckI /\ trans l  (communicating P Q) P') \/
-       (l = val tt /\ P' ≅ stuckI /\ trans l' (communicating P Q) Q')
-    ).
+    trans l (communicating P Q) (communicating P' Q).
 Proof.
   intros * TRP TRQ.
-  destruct l, l'.
-  - left.
-    apply trans_get_head in TRP.
+  destruct l, l';
+  try (pose proof (trans_val_invT TRP); subst; easy);
+    try (pose proof (trans_val_invT TRQ); subst; easy).
+  - apply trans_get_head in TRP.
     apply trans_get_head in TRQ.
     destruct TRP as (? & ? & ? & TRP & EQP).
     destruct TRQ as (? & ? & ? & TRQ & EQQ).
@@ -446,8 +853,7 @@ Proof.
     eapply (trans_ChoiceI Fin.F1); [| reflexivity].
     rewrite EQP.
     pose proof (@trans_ChoiceV _ _ x (fun i : fin x => communicating (x0 i) Q) x1); auto.
-  - left.
-    apply trans_get_head in TRP.
+  - apply trans_get_head in TRP.
     apply trans_get_head in TRQ.
     destruct TRP as (? & ? & ? & TRP & EQP).
     destruct TRQ as (? & TRQ & EQQ).
@@ -457,18 +863,7 @@ Proof.
     eapply (trans_ChoiceI Fin.F1); [| reflexivity].
     rewrite EQP.
     pose proof (@trans_ChoiceV _ _ x (fun i : fin x => communicating (x0 i) Q) x1); auto.
-  - right; left.
-    destruct (trans_get_head TRP) as (? & ? & ? & TRP' & EQP).
-    pose proof (trans_val_invT TRQ); subst X; destruct v.
-    apply trans_get_head in TRQ.
-    destruct TRQ as (TRQ & EQQ).
-    do 2 split; auto.
-    rewrite unfold_communicating.
-    cbn in *.
-    do 2 (eapply trans_bind_r; [cbn; eauto |]); cbn.
-    auto.
-  - left.
-    apply trans_get_head in TRP.
+  - apply trans_get_head in TRP.
     apply trans_get_head in TRQ.
     destruct TRP as (? & TRP & EQP).
     destruct TRQ as (? & ? & ? & TRQ & EQQ).
@@ -478,15 +873,14 @@ Proof.
     eapply (trans_ChoiceI Fin.F1); [| reflexivity].
     constructor.
     rewrite EQP; auto.
-  - left.
-    apply trans_get_head in TRP.
+  - apply trans_get_head in TRP.
     apply trans_get_head in TRQ.
     destruct TRP as (? & TRP & EQP).
     destruct TRQ as (? & TRQ & EQQ).
     rewrite unfold_communicating.
     cbn in *.
     do 2 (eapply trans_bind_r; [cbn; eauto |]); cbn.
-    destruct e, e0. 
+    destruct e, e0.
     destruct (are_opposite a a0).
     + eapply (trans_ChoiceI (Fin.FS Fin.F1)); [| reflexivity].
       rewrite EQP.
@@ -496,58 +890,19 @@ Proof.
       rewrite EQP.
       repeat match goal with | h : unit |- _ => destruct h end.
       eapply trans_trigger'.
-  - right; left.
-    destruct (trans_get_head TRP) as (? & TRP' & EQP).
-    pose proof (trans_val_invT TRQ); subst; destruct v0.
-    apply trans_get_head in TRQ.
-    destruct TRQ as (TRQ & EQQ).
-    do 2 split; auto.
-    rewrite unfold_communicating.
-    cbn in *.
-    do 2 (eapply trans_bind_r; [cbn; eauto |]); cbn.
-    destruct e; auto.
-  - right; right.
-    pose proof (trans_val_invT TRP); subst; destruct v.
-    destruct (trans_get_head TRP) as (TRP' & EQP).
-    destruct (trans_get_head TRQ) as (? & ? & ? & TRQ' & EQQ).
-    do 2 split; auto.
-    rewrite unfold_communicating.
-    cbn in *.
-    do 2 (eapply trans_bind_r; [cbn; eauto |]); cbn; auto.
-  - (* We cannot if P returns *)
-    right; right.
-    pose proof (trans_val_invT TRP); subst; destruct v.
-    destruct (trans_get_head TRP) as (TRP' & EQP).
-    destruct (trans_get_head TRQ) as (? & TRQ' & EQQ).
-    do 2 split; auto.
-    rewrite unfold_communicating.
-    cbn in *.
-    do 2 (eapply trans_bind_r; [cbn; eauto |]); cbn; auto.
-   - (* We cannot if P returns *)
-    right; right.
-    pose proof (trans_val_invT TRP); subst; destruct v.
-    destruct (trans_get_head TRP) as (TRP' & EQP).
-    pose proof (trans_val_invT TRQ); subst; destruct v0.
-    destruct (trans_get_head TRQ) as (TRQ' & EQQ).
-    do 2 split; auto.
-    rewrite unfold_communicating.
-    cbn in *.
-    do 2 (eapply trans_bind_r; [cbn; eauto |]); cbn; auto.
- Qed.
+Qed.
 
 Lemma trans_communicatingR :
   forall l l' (P P' Q Q' : ccs),
     trans l P P' ->
     trans l' Q Q' ->
-    (trans l' (communicating P Q) (communicating P Q') \/
-       (l = val tt /\ P' ≅ stuckI /\ trans l' (communicating P Q) Q') \/
-       (l' = val tt /\ Q' ≅ stuckI /\ trans l (communicating P Q) P')
-    ).
+    trans l' (communicating P Q) (communicating P Q').
 Proof.
   intros * TRP TRQ; cbn in *.
-  destruct l, l'.
-  - left.
-    apply trans_get_head in TRP.
+  destruct l, l';
+    try (pose proof (trans_val_invT TRP); subst; easy);
+    try (pose proof (trans_val_invT TRQ); subst; easy).
+  - apply trans_get_head in TRP.
     apply trans_get_head in TRQ.
     destruct TRP as (? & ? & ? & TRP & EQP).
     destruct TRQ as (? & ? & ? & TRQ & EQQ).
@@ -557,8 +912,7 @@ Proof.
     eapply (trans_ChoiceI (Fin.FS Fin.F1)); [| reflexivity].
     rewrite EQQ.
     pose proof (@trans_ChoiceV _ _ x2 (fun i : fin x2 => communicating P (x3 i)) x4); auto.
-  - left.
-    apply trans_get_head in TRP.
+  - apply trans_get_head in TRP.
     apply trans_get_head in TRQ.
     destruct TRP as (? & ? & ? & TRP & EQP).
     destruct TRQ as (? & TRQ & EQQ).
@@ -567,24 +921,14 @@ Proof.
     do 2 (eapply trans_bind_r; [cbn; eauto |]); cbn.
     eapply (trans_ChoiceI (Fin.FS Fin.F1)); [| reflexivity].
     constructor; rewrite EQQ; auto.
-  - right; right.
-    pose proof (trans_val_invT TRQ); subst; destruct v.
-    destruct (trans_get_head TRP) as (? & ? & ? & TRP' & EQP).
-    destruct (trans_get_head TRQ) as (TRQ' & EQQ).
-    do 2 split; auto.
-    rewrite unfold_communicating.
-    cbn in *.
-    do 2 (eapply trans_bind_r; [cbn; eauto |]); cbn; auto.
-  - left.
-    destruct (trans_get_head TRP) as (? & TRP' & EQP).
+  - destruct (trans_get_head TRP) as (? & TRP' & EQP).
     destruct (trans_get_head TRQ) as (? & ? & ? & TRQ' & EQQ).
     rewrite unfold_communicating.
     cbn in *.
     do 2 (eapply trans_bind_r; [cbn; eauto |]); cbn; auto.
     eapply (trans_ChoiceI (Fin.FS Fin.F1)); [| reflexivity].
     rewrite EQQ; econstructor; auto.
-  - left.
-    destruct (trans_get_head TRP) as (? & TRP' & EQP).
+  - destruct (trans_get_head TRP) as (? & TRP' & EQP).
     destruct (trans_get_head TRQ) as (? & TRQ' & EQQ).
     rewrite unfold_communicating.
     cbn in *.
@@ -599,134 +943,106 @@ Proof.
       rewrite EQQ.
       repeat match goal with | h : unit |- _ => destruct h end.
       eapply trans_trigger'.
-  - right; right.
-    pose proof (trans_val_invT TRQ); subst; destruct v0.
-    destruct (trans_get_head TRP) as (? & TRP' & EQP).
-    destruct (trans_get_head TRQ) as (TRQ' & EQQ).
-    do 2 split; auto.
-    rewrite unfold_communicating.
-    cbn in *.
-    do 2 (eapply trans_bind_r; [cbn; eauto |]); cbn; auto.
-  - right; left.
-    pose proof (trans_val_invT TRP); subst; destruct v.
-    destruct (trans_get_head TRP) as (TRP' & EQP).
-    destruct (trans_get_head TRQ) as (? & ? & ? & TRQ' & EQQ).
-    do 2 split; auto.
-    rewrite unfold_communicating.
-    cbn in *.
-    do 2 (eapply trans_bind_r; [cbn; eauto |]); cbn; auto.
-  - right; left.
-    pose proof (trans_val_invT TRP); subst; destruct v.
-    destruct (trans_get_head TRP) as (TRP' & EQP).
-    destruct (trans_get_head TRQ) as (? & TRQ' & EQQ).
-    do 2 split; auto.
-    rewrite unfold_communicating.
-    cbn in *.
-    do 2 (eapply trans_bind_r; [cbn; eauto |]); cbn; auto.
-  - right; left.
-    pose proof (trans_val_invT TRP); subst; destruct v.
-    pose proof (trans_val_invT TRQ); subst; destruct v0.
-    destruct (trans_get_head TRP) as (TRP' & EQP).
-    destruct (trans_get_head TRQ) as (TRQ' & EQQ).
-    do 2 split; auto.
-    rewrite unfold_communicating.
-    cbn in *.
-    do 2 (eapply trans_bind_r; [cbn; eauto |]); cbn; auto.
 Qed.
 
-Notation "0" := nil: ccs_scope.
-Infix "+" := plus (at level 50, left associativity).
-Infix "∥" := communicating (at level 29, left associativity).
+Ltac clear_tt :=
+  repeat match goal with
+  | h : unit |- _ => destruct h
+  end.
 
-Section Theory.
+Lemma trans_communicating_inv :
+  forall l p q r,
+    trans l (communicating p q) r ->
+    (exists p' q' l', trans l p p' /\ trans l' q q' /\ r ≅ (communicating p' q)) \/
+      (exists q' p' l', trans l q q' /\ trans l' p p' /\ r ≅ (communicating p q')) \/
+      (exists p' q' a b,
+          trans (comm a) p p' /\
+            trans (comm b) q q' /\
+            are_opposite a b /\
+            r ≅ (communicating p' q')).
+Proof.
+  (*
+  intros * TR.
+  rewrite unfold_communicating in TR.
+  edestruct @trans_bind_inv; [apply TR | | ]; clear TR.
+  destruct H as (NOTV & ? & TR & EQ); apply trans_get_head_inv in TR; easy.
+  destruct H as (hdP & TRhdP & TR).
+  edestruct @trans_bind_inv; [apply TR | | ]; clear TR.
+  destruct H as (NOTV & ? & TR & EQ); apply trans_get_head_inv in TR; easy.
+  destruct H as (hdQ & TRhdQ & TR).
+  destruct hdP; try easy.
+  + destruct hdQ; try easy.
+    *
+      inv_trans.
+      { apply trans_ChoiceV_inv in TR as (x & EQ & ->).
 
-  Lemma plsC: forall (p q : ccs), p+q ~ q+p.
-  Proof.
-    apply choiceI2_commut.
-  Qed.
+      inv_trans;
+        apply trans_ChoiceV_inv in TR as (x & EQ & ->);
+        eapply trans_HChoice in TRhdP;
+        eapply trans_HChoice in TRhdQ;
+        eauto 8.
+    * inv_trans;
+        ( apply trans_ChoiceV_inv in TR as (x & EQ & ->) ||
+          apply trans_vis_inv in TR as (x & EQ & ->));
+          eapply trans_HChoice in TRhdP;
+          eapply trans_HVis in TRhdQ;
+          eauto 8.
+  + destruct hdQ.
+    * apply trans_HRet in TRhdQ; destruct r0.
+    * inv_trans;
+        ( apply trans_ChoiceV_inv in TR as (x & EQ & ->) ||
+          apply trans_vis_inv in TR as (x & EQ & ->));
+        eapply trans_HVis in TRhdP;
+          eapply trans_HChoice in TRhdQ;
+        eauto 8.
+    * destruct e, e0.
+      destruct (are_opposite a a0) eqn:OP; inv_trans.
+      all: ( apply trans_ChoiceV_inv in TR as (x & EQ & ->) ||
+             apply trans_trigger_inv in TR as (x & EQ & ->)).
+      all: eapply trans_HVis in TRhdP;
+        eapply trans_HVis in TRhdQ.
+      all: clear_tt.
+      all: eauto 12.
 
-  Lemma plsA (p q r : ccs): p+(q+r) ~ (p+q)+r.
-  Proof.
-    symmetry; apply choiceI2_assoc.
-  Qed.
+      right; right; eauto 8.
+      left.
+      { repeat right.
+        apply trans_ChoiceV_inv in TR.
+        destruct TR as (x & EQ & ->).
+        do 4 eexists; repeat split; eauto.
+        eapply trans_HVis in TRhdP; apply TRhdP.
+        eapply trans_HVis in TRhdQ; apply TRhdQ.
+      }
+      { left.
+        apply trans_trigger_inv in TR.
+        destruct TR as (x & -> & EQ).
+        eexists; split; eauto.
+        eapply trans_HVis in TRhdP.
+        destruct x; apply TRhdP.
+      }
+      { right; left.
+        apply trans_trigger_inv in TR.
+        destruct TR as (x & -> & EQ).
+        eexists; split; eauto.
+        eapply trans_HVis in TRhdQ.
+        destruct x; apply TRhdQ.
+      }
+      { left.
+        apply trans_trigger_inv in TR.
+        destruct TR as (x & -> & EQ).
+        eexists; split; eauto.
+        eapply trans_HVis in TRhdP.
+        destruct x; apply TRhdP.
+      }
+      { right; left.
+        apply trans_trigger_inv in TR.
+        destruct TR as (x & -> & EQ).
+        eexists; split; eauto.
+        eapply trans_HVis in TRhdQ.
+        destruct x; apply TRhdQ.
+      }
+Qed.
 
-  Lemma pls0p (p : ccs) : 0 + p ~ p.
-  Proof.
-    apply choiceI2_stuckV_l.
-  Qed.
+   *)
+Admitted.
 
-  Lemma plsp0 (p : ccs) : p + 0 ~ p.
-  Proof. now rewrite plsC, pls0p. Qed.
-
-  Lemma plsidem (p : ccs) : p + p ~ p.
-  Proof.
-    apply choiceI2_idem.
-  Qed.
-
-  Lemma paraC: forall (p q : ccs), p ∥ q ~ q ∥ p.
-  Proof.
-    coinduction ? CIH; symmetric.
-    intros p q l r tr.
-    cbn in *.
-    rewrite unfold_communicating in tr.
-  Admitted.
-
-  Lemma para0p : forall (p : ccs), 0 ∥ p ~ p.
-  Proof.
-  Admitted.
-
-  Lemma commC: forall (p q : ccs), p ∥ q ~ q ∥ p.
-  Proof.
-  Admitted.
-
-End Theory.
-
-Import CCSNotations.
-Open Scope ccs_scope.
-
-(* fun P Q => bisim (model P) (model Q): is this weak bisimulation of CCS?
-
-   -> : term -> term -> Prop
-   -ccs> : ccs -> ccs -> Prop as
-   -sem> : term -> term -> Prop := fun P Q => model P -ccs> model Q
-*)
-
-Fixpoint model (t : term) : ccs :=
-	match t with
-	| 0      => nil
-	| a · P  => prefix a (model P)
-	| TauT P => TauV (model P)
-	| P ∥ Q  => communicating (model P) (model Q)
-	| P ⊕ Q  => plus (model P) (model Q)
-	| P ∖ c  => restrict c (model P)
-	end.
-
-(*
-Variant step_ccs : ccs -> option action -> ccs -> Prop :=
-| Sted_comm : forall (t : ccs) a u k,
-	schedule t u ->
-  u ≅ trigger (Act a);; k ->
-	step_ccs t (Some a) k
-| Step_tau : forall (t : ccs) u k,
-	schedule t u ->
-  u ≅ trigger Tau;; k ->
-	step_ccs t None k.
-
-Definition step_sem : term -> option action -> term -> Prop :=
-	fun P a Q => step_ccs (model P) a (model Q).
-*)
-
-Module DenNotations.
-
-  (* Notations for patterns *)
-  Notation "'synchP' e" := (inl1 e) (at level 10).
-  Notation "'actP' e" := (inr1 (inl1 e)) (at level 10).
-  Notation "'deadP' e" :=  (inr1 (inr1 e)) (at level 10).
-
-  Notation "⟦ t ⟧" := (model t).
-  (* Notation "P '⊢' a '→ccs' Q" := (step_ccs P a Q) (at level 50). *)
-  (* Notation "P '⊢' a '→sem' Q" := (step_sem P a Q) (at level 50). *)
-
-End DenNotations.
-
-Import DenNotations.
